lean/src/internal/gdt_hom.lean
@@ -1,0 +1,58 @@
+import tactic
+import ..definitions
+import .gdt_stable
+import data.finset
+
+variable [GuardModule]
+open GuardModule
+
+def homomorphic (f: Φ → Φ) := ∀ ty1 ty2: Φ, (f (ty1.or ty2)).eval = ((f ty1).or (f ty2)).eval
+
+lemma id_hom: homomorphic id := begin
+    simp [homomorphic],
+end
+
+lemma and_right_hom { ty: Φ }: homomorphic ty.and :=
+begin
+    rw homomorphic,
+    assume ty1 ty2,
+    ext env,
+    cases c1: ty.eval env;
+    cases c2: ty1.eval env;
+    cases c3: ty2.eval env;
+    simp [*, Φ.eval],
+end
+
+lemma or_right_hom { ty: Φ }: homomorphic ty.or :=
+begin
+    rw homomorphic,
+    assume ty1 ty2,
+    ext env,
+    cases c1: ty.eval env;
+    cases c2: ty1.eval env;
+    cases c3: ty2.eval env;
+    simp [*, Φ.eval],
+end
+
+lemma xgrd_in_hom (grd: XGrd): homomorphic (Φ.xgrd_in grd) :=
+begin
+    rw homomorphic,
+    assume ty1 ty2,
+    ext env,
+    cases c: xgrd_eval grd env;
+    simp [*, Φ.eval],
+end
+
+lemma comp_hom { f1 f2: Φ → Φ } (f1_hom: homomorphic f1) (f1_stable: stable f1) (f2_hom: homomorphic f2) (f2_stable: stable f2): homomorphic (f1 ∘ f2) :=
+begin
+    unfold homomorphic,
+    assume ty1 ty2,
+    unfold function.comp,
+    
+    have : (f2 (ty1.or ty2)).eval = ((f2 ty1).or (f2 ty2)).eval := begin
+      simp [f2_hom _ _],
+    end,
+
+    rw stable_app f1_stable this,
+    rw f1_hom,
+end
