lean/src/internal/helper_defs.lean
@@ -1,0 +1,149 @@
+import tactic
+import ..definitions
+import .gdt_stable
+import .gdt_hom
+import data.finset
+
+variable [GuardModule]
+open GuardModule
+
+-- Simpler definition of 𝒰 that does not need an accumulator
+def U : Gdt → Φ
+| (Gdt.leaf _) := Φ.false
+| (Gdt.branch tr1 tr2) := (U tr1).and (U tr2)
+| (Gdt.grd (Grd.bang var) tree) := ((Φ.var_is_not_bottom var).and (U tree))
+| (Gdt.grd (Grd.xgrd grd) tree) :=
+                (Φ.not_xgrd grd)
+            .or
+                (Φ.xgrd_in grd (U tree))
+
+lemma U_eq_𝒰_acc { gdt: Gdt } { acc: Φ → Φ } (acc_stable: stable acc) (acc_hom: homomorphic acc) : (acc (U gdt)).eval = (𝒰_acc acc gdt).eval :=
+begin
+    induction gdt generalizing acc,
+    
+    case Gdt.leaf {
+        simp [𝒰_acc, U],
+    },
+
+    case Gdt.branch {
+        have : (𝒰_acc id gdt_tr1).eval = (id (U gdt_tr1)).eval := begin
+            simp [←gdt_ih_tr1, id_stable, id_hom],
+        end,
+        have : ((𝒰_acc id gdt_tr1).and (U gdt_tr2)).eval = ((id (U gdt_tr1)).and (U gdt_tr2)).eval := begin
+            rw stable_app and_left_stable this,
+        end,
+        simp [𝒰_acc, U, ←gdt_ih_tr2 (stable_comp acc_stable and_right_stable) (comp_hom acc_hom acc_stable and_right_hom and_right_stable),
+            function.comp, stable_app acc_stable this],
+    },
+
+    case Gdt.grd {
+        cases gdt_grd,
+        
+        case Grd.xgrd {
+            ext env,
+            simp [𝒰_acc, U],
+            rw acc_hom,
+            have : (𝒰_acc (acc ∘ Φ.xgrd_in gdt_grd) gdt_tr).eval = (acc (Φ.xgrd_in gdt_grd (U gdt_tr))).eval := begin
+                simp [←gdt_ih (stable_comp acc_stable (xgrd_in_stable _))
+                    (comp_hom acc_hom acc_stable (xgrd_in_hom gdt_grd) (xgrd_in_stable gdt_grd))],
+            end,
+            rw stable_app or_right_stable this,
+        },
+
+        case Grd.bang {
+            simp [𝒰_acc, U, ←gdt_ih (stable_comp acc_stable and_right_stable) (comp_hom acc_hom acc_stable and_right_hom and_right_stable)],
+        },
+    },
+end
+
+lemma U_eq_𝒰 (gdt: Gdt) : (U gdt).eval = (𝒰 gdt).eval :=
+begin
+    ext env,
+    simp [𝒰, ←U_eq_𝒰_acc (id_stable) (id_hom)],
+end
+
+
+def Ant.map { α : Type } { β : Type } : (α → β) → Ant α → Ant β
+| f (Ant.leaf a leaf) := Ant.leaf (f a) leaf
+| f (Ant.branch tr1 tr2) := (Ant.branch (tr1.map f) (tr2.map f))
+| f (Ant.diverge a tr) := (Ant.diverge (f a) (tr.map f))
+
+def Ant.map_option { α : Type } { β : Type } : (α → β) → option (Ant α) → option (Ant β)
+| f (some ant) := some (ant.map f)
+| f none := none
+
+def Ant.eval_leaves (ant: Ant Φ) (env: Env) := ant.map (λ ty, ty.eval env)
+
+-- This is a simpler definition of 𝒜 that is semantically equivalent.
+def A : Gdt → Ant Φ
+| (Gdt.leaf leaf) := Ant.leaf Φ.true leaf
+| (Gdt.branch tr1 tr2) := Ant.branch (A tr1) $ (A tr2).map ((U tr1).and)
+| (Gdt.grd (Grd.bang var) tr) := Ant.diverge (Φ.var_is_bottom var) $ (A tr).map ((Φ.var_is_not_bottom var).and)
+| (Gdt.grd (Grd.xgrd grd) tr) := (A tr).map (Φ.xgrd_in grd)
+
+def Ant.leaves { α: Type }: Ant α → finset Leaf
+| (Ant.leaf a leaf) := { leaf }
+| (Ant.branch tr1 tr2) := Ant.leaves tr1 ∪ Ant.leaves tr2
+| (Ant.diverge a tr) := Ant.leaves tr
+
+
+-- (accessible, inaccessible, redundant)
+structure LeafPartition := mk :: (acc : list Leaf) (inacc : list Leaf) (red : list Leaf)
+
+def R' : Ant bool → LeafPartition
+| (Ant.leaf can_prove_empty n) := if can_prove_empty then ⟨ [], [], [n] ⟩ else ⟨ [n], [], [] ⟩
+| (Ant.diverge can_prove_empty tr) := 
+    match R' tr, can_prove_empty with
+    | ⟨ [], [], m :: ms ⟩, ff := ⟨ [], [m], ms ⟩
+    | r, _ := r
+    end
+| (Ant.branch tr1 tr2) :=
+    let r1 := R' tr1, r2 := R' tr2 in
+        ⟨ r1.acc ++ r2.acc, r1.inacc ++ r2.inacc, r1.red ++ r2.red ⟩
+
+/-
+    This definition is much easier to use than ℛ, but equal to ℛ.
+    * Associativity of `Ant.map` can be utilized.
+    * LeafPartition is much easier to use than triples.
+    * Ant.branch has no match which would require a case distinction.
+-/
+def R (can_prove_empty: Φ → bool) (ant: Ant Φ): LeafPartition := R' (ant.map can_prove_empty)
+
+def to_triple (p: LeafPartition): (list Leaf × list Leaf × list Leaf) :=
+    (p.acc, p.inacc, p.red)
+
+lemma R_eq_ℛ (can_prove_empty: Φ -> bool) (ant: Ant Φ): to_triple (R can_prove_empty ant) = ℛ can_prove_empty ant :=
+begin
+    induction ant,
+    case Ant.leaf {
+        cases c: can_prove_empty ant_a;
+        simp [R, R', R'._match_1, ℛ, ℛ._match_1, Ant.map, ℛ._match_2, to_triple, c],
+    },
+    
+    case Ant.branch {
+        rw ℛ,
+        rw ←ant_ih_tr1,
+        rw ←ant_ih_tr2,
+        
+        cases ℛ can_prove_empty ant_tr1 with a1 ir1;
+        cases ir1 with i1 r1;
+        cases ℛ can_prove_empty ant_tr2 with a2 ir2;
+        cases ir2 with i2 r2;
+
+        simp [R, R', R'._match_1, ℛ, ℛ._match_1, Ant.map, ℛ._match_2, to_triple],
+    },
+
+    case Ant.diverge {
+        rw ℛ,
+        rw ←ant_ih,
+
+        cases c1: can_prove_empty ant_a;
+        cases c: (R' (Ant.map can_prove_empty ant_tr));
+        cases acc;
+        cases inacc;
+        cases red;
+
+        simp [R, R', R'._match_1, ℛ, ℛ._match_1, Ant.map, ℛ._match_2, to_triple, c1, c],
+    },
+end
+
