lean/src/internal/leaves_theory.lean
@@ -1,0 +1,27 @@
+
+import tactic
+import ..definitions
+import data.finset
+
+variable [GuardModule]
+open GuardModule
+
+
+
+@[simp]
+lemma map_leaves_id { α: Type } { β: Type } (ant: Ant α) (f: α → β): ant_leaves (map_ant f ant) = ant_leaves ant :=
+begin
+    induction ant;
+    finish [ant_leaves, map_ant],
+end
+
+lemma gdt_leaves_eq_ant_leaves (gdt: Gdt): ant_leaves (𝒜' gdt) = gdt_leaves gdt :=
+begin
+    induction gdt,
+    case Gdt.leaf { finish, },
+    case Gdt.branch { finish [gdt_leaves, ant_leaves, 𝒜', map_ant], },
+    case Gdt.grd {
+        cases gdt_grd;
+        finish [gdt_leaves, ant_leaves, 𝒜', map_ant],
+    },
+end
