lean/src/internal/utils.lean
@@ -1,0 +1,11 @@
+
+import tactic
+import data.finset
+
+lemma to_finset_append { α: Type } [decidable_eq α] { l1: list α } { l2: list α }:
+    (l1 ++ l2).to_finset = l1.to_finset ∪ l2.to_finset :=
+begin
+    induction l1;
+    finish,
+end
+
